add new SymCC primitives for comparing the matches-behavior of individual policies
Signed-off-by: Craig Disselkoen <cdiss@amazon.com>

cedar-lean/Cedar/SymCC.lean
@@ -182,7 +182,7 @@ def alwaysMatches? (p : Policy) (εnv : SymEnv) : SolverM (Option Env) :=
 Returns `none` iff `p` matches no well-formed inputs in `εnv`.
 Otherwise returns an input `some env` that is matched by `p`.
 
-Compare with `alwaysDenies`, which takes a policyset (which could consist of a
+Compare with `alwaysDenies?`, which takes a policyset (which could consist of a
 single policy, or more) and determines whether it _denies_ all well-formed
 inputs in an `εnv`. This function differs from `alwaysDenies` on a singleton
 policyset in how it treats `forbid` policies -- while `alwaysDenies` trivially
@@ -191,6 +191,58 @@ holds if the `forbid` policy explicitly denies no inputs in the `εnv`.
 -/
 def neverMatches? (p : Policy) (εnv : SymEnv) : SolverM (Option Env) :=
   sat? [p] (verifyNeverMatches p) εnv
+
+/--
+Returns `none` iff `p₁` and `p₂` match exactly the same set of well-formed
+inputs in `εnv`.  Otherwise returns an input `some env` on which `p₁` and `p₂`
+have different matching behavior (one matches and the other does not).
+
+Compare with `equivalent?`, which takes two policysets (which could consist of a
+single policy, or more) and determines whether the _authorization behavior_ of
+those policysets is equivalent for well-formed inputs in `εnv`. This function
+differs from `equivalent?` on singleton policysets in how it treats `forbid`
+policies -- while `equivalent?` trivially holds for any pair of `forbid` policies
+(as they both always-deny), `matchesEquivalent?` only holds if the two policies
+match exactly the same set of inputs. Also, a nontrivial `permit` and nontrivial
+`forbid` policy can be `matchesEquivalent?`, but can never be `equivalent?`.
+-/
+def matchesEquivalent? (p₁ p₂ : Policy) (εnv : SymEnv) : SolverM (Option Env) :=
+  sat? [p₁, p₂] (verifyMatchesEquivalent p₁ p₂) εnv
+
+/--
+Returns `none` iff `p₁` matching implies that `p₂` matches, for every
+well-formed input in `εnv`. That is, for every request where `p₁` matches, `p₂`
+also matches. Otherwise returns an input `some env` that is matched by `p₁` but
+not-matched by `p₂`.
+
+Compare with `implies?`, which takes two policysets (which could consist of a
+single policy, or more) and determines whether the _authorization decision_ of
+the first implies that of the second. This function differs from `implies?` on
+singleton policysets in how it treats `forbid` policies -- while for `implies?`,
+any `forbid` policy trivially implies any `permit` policy (as always-deny always
+implies any policy), for `matchesImplies?`, a `forbid` policy may or may not
+imply a `permit` policy, and a `permit` policy may or may not imply a `forbid`
+policy.
+-/
+def matchesImplies? (p₁ p₂ : Policy) (εnv : SymEnv) : SolverM (Option Env) :=
+  sat? [p₁, p₂] (verifyMatchesImplies p₁ p₂) εnv
+
+/--
+Returns `none` iff there is no well-formed input in `εnv` that is matched by
+both `p₁` and `p₂`. Otherwise returns an input `some env` that is matched by
+both `p₁` and `p₂`. This checks that the sets of inputs matched by `p₁` and `p₂`
+are disjoint.
+
+Compare with `disjoint?`, which takes two policysets (which could consist of a
+single policy, or more) and determines whether the _authorization behavior_ of
+those policysets are disjoint. This function differs from `disjoint?` on
+singleton policysets in how it treats `forbid` policies -- while for
+`disjoint?`, any `forbid` policy is trivially disjoint from any other policy (as
+it allows nothing), `matchesDisjoint?` considers whether the `forbid` policy may
+_match_ (rather than _allow_) any input that is matched by the other policy.
+-/
+def matchesDisjoint? (p₁ p₂ : Policy) (εnv : SymEnv) : SolverM (Option Env) :=
+  sat? [p₁, p₂] (verifyMatchesDisjoint p₁ p₂) εnv
 
 /--
 Returns `none` iff the authorization decision of `ps₁` implies that of `ps₂` for
@@ -302,6 +354,56 @@ denies no inputs in the `εnv`.
 -/
 def checkNeverMatches (p : Policy) (εnv : SymEnv) : SolverM Bool :=
   checkUnsat (verifyNeverMatches p) εnv
+
+/--
+Returns true iff `p₁` and `p₂` match exactly the same set of well-formed
+inputs in `εnv`.
+
+Compare with `checkEquivalent`, which takes two policysets (which could consist of a
+single policy, or more) and determines whether the _authorization behavior_ of
+those policysets is equivalent for well-formed inputs in `εnv`. This function
+differs from `checkEquivalent` on a singleton policyset in how it treats `forbid`
+policies -- while `checkEquivalent` trivially holds for any pair of `forbid` policies
+(as they both always-deny), `checkMatchesEquivalent` only holds if the two policies
+match exactly the same set of inputs. Also, a nontrivial `permit` and nontrivial
+`forbid` policy can be `checkMatchesEquivalent`, but can never be `checkEquivalent`.
+-/
+def checkMatchesEquivalent (p₁ p₂ : Policy) (εnv : SymEnv) : SolverM Bool :=
+  checkUnsat (verifyMatchesEquivalent p₁ p₂) εnv
+
+/--
+Returns true iff `p₁` matching implies that `p₂` matches, for every
+well-formed input in `εnv`. That is, for every request where `p₁` matches, `p₂`
+also matches.
+
+Compare with `checkImplies`, which takes two policysets (which could consist of
+a single policy, or more) and determines whether the _authorization decision_ of
+the first implies that of the second. This function differs from `checkImplies`
+on singleton policysets in how it treats `forbid` policies -- while for
+`checkImplies`, any `forbid` policy trivially implies any `permit` policy (as
+always-deny always implies any policy), for `checkMatchesImplies`, a `forbid`
+policy may or may not imply a `permit` policy, and a `permit` policy may or may
+not imply a `forbid` policy.
+-/
+def checkMatchesImplies (p₁ p₂ : Policy) (εnv : SymEnv) : SolverM Bool :=
+  checkUnsat (verifyMatchesImplies p₁ p₂) εnv
+
+/--
+Returns true iff there is no well-formed input in `εnv` that is matched by
+both `p₁` and `p₂`. This checks that the sets of inputs matched by `p₁` and `p₂`
+are disjoint.
+
+Compare with `checkDisjoint`, which takes two policysets (which could consist of
+a single policy, or more) and determines whether the _authorization behavior_ of
+those policysets are disjoint. This function differs from `checkDisjoint` on
+singleton policysets in how it treats `forbid` policies -- while for
+`checkDisjoint`, any `forbid` policy is trivially disjoint from any other policy
+(as it allows nothing), `checkMatchesDisjoint` considers whether the `forbid`
+policy may _match_ (rather than _allow_) any input that is matched by the other
+policy.
+-/
+def checkMatchesDisjoint (p₁ p₂ : Policy) (εnv : SymEnv) : SolverM Bool :=
+  checkUnsat (verifyMatchesDisjoint p₁ p₂) εnv
 
 /--
 Returns true iff the authorization decision of `ps₁` implies that of `ps₂` for
