cedar-lean/Cedar/Thm/SymCC/Verifier/VerifyEvaluatePair.lean
@@ -1,0 +1,192 @@
+/-
+ Copyright Cedar Contributors
+
+ Licensed under the Apache License, Version 2.0 (the "License");
+ you may not use this file except in compliance with the License.
+ You may obtain a copy of the License at
+
+      https://www.apache.org/licenses/LICENSE-2.0
+
+ Unless required by applicable law or agreed to in writing, software
+ distributed under the License is distributed on an "AS IS" BASIS,
+ WITHOUT WARRANTIES OR CONDITIONS OF ANY KIND, either express or implied.
+ See the License for the specific language governing permissions and
+ limitations under the License.
+-/
+
+import Cedar.SymCC.Verifier
+import Cedar.Thm.SymCC.Enforcer
+import Cedar.Thm.SymCC.Authorizer
+import Cedar.Thm.SymCC.Verifier.Same
+
+/-!
+This file proves the soundness and completeness of
+`Cedar.SymCC.verifyEvaluatePair` for well-behaved verification queries.  This
+enables proving soundness and completeness of analyses built on `verifyEvaluatePair`
+by proving that their queries are well-behaved.
+--/
+
+namespace Cedar.Thm
+
+open Data Spec SymCC Factory
+
+def WellBehavedEvaluatePairQuery (φ : Term → Term → Term) (f : Spec.Result Value → Spec.Result Value → Bool) : Prop :=
+  WellFormedOutput ∧ Interpretable ∧ Same
+where
+  WellFormedInput (t₁ t₂ : Term) (εs : SymEntities) :=
+    t₁.WellFormed εs ∧ t₁.typeOf = .option .bool ∧
+    t₂.WellFormed εs ∧ t₂.typeOf = .option .bool
+  WellFormedOutput :=
+    ∀ (t₁ t₂ : Term) (εs : SymEntities),
+      WellFormedInput t₁ t₂ εs →
+      (φ t₁ t₂).WellFormed εs ∧ (φ t₁ t₂).typeOf = .bool
+  Interpretable :=
+    ∀ (t₁ t₂ : Term) (εs : SymEntities) (I : Interpretation),
+      WellFormedInput t₁ t₂ εs →
+      I.WellFormed εs →
+      (φ t₁ t₂).interpret I = φ (t₁.interpret I) (t₂.interpret I)
+  Same :=
+    ∀ (t₁ t₂ : Term) (εs : SymEntities) (r₁ r₂ : Spec.Result Value),
+      WellFormedInput t₁ t₂ εs →
+      r₁ ∼ t₁ →
+      r₂ ∼ t₂ →
+      (f r₁ r₂) ∼ (φ t₁ t₂)
+
+private theorem wbepq_bisimulation {φ : Term → Term → Term} {f : Spec.Result Value → Spec.Result Value → Bool} {εs : SymEntities} {t₁ t₂ : Term} {r₁ r₂ : Spec.Result Value} {I : Interpretation} :
+  WellBehavedEvaluatePairQuery.WellFormedInput t₁ t₂ εs →
+  WellBehavedEvaluatePairQuery.Same φ f →
+  I.WellFormed εs →
+  r₁ ∼ (t₁.interpret I) →
+  r₂ ∼ (t₂.interpret I) →
+  (f r₁ r₂) ∼ (φ (t₁.interpret I) (t₂.interpret I))
+:= by
+  intro hwt hφf hwI heq₁ heq₂
+  have hwt₁' := interpret_term_wf hwI hwt.left
+  have hwt₂' := interpret_term_wf hwI hwt.2.2.left
+  have hwt₁_wf := hwt₁'.left
+  have hwt₁_ty := hwt₁'.right
+  have hwt₂_wf := hwt₂'.left
+  have hwt₂_ty := hwt₂'.right
+  rw [hwt.2.left] at hwt₁_ty
+  rw [hwt.2.2.2] at hwt₂_ty
+  exact hφf (t₁.interpret I) (t₂.interpret I) εs r₁ r₂ ⟨hwt₁_wf, hwt₁_ty, hwt₂_wf, hwt₂_ty⟩ heq₁ heq₂
+
+private theorem interpret_not_wbepq {φ : Term → Term → Term} {t₁ t₂ : Term} {I : Interpretation} {εs : SymEntities} :
+  I.WellFormed εs →
+  WellBehavedEvaluatePairQuery.WellFormedInput t₁ t₂ εs →
+  WellBehavedEvaluatePairQuery.WellFormedOutput φ →
+  WellBehavedEvaluatePairQuery.Interpretable φ →
+  Term.interpret I (not (φ t₁ t₂)) = not (φ (t₁.interpret I) (t₂.interpret I))
+:= by
+  intro hwI hwt hwφ hiφ
+  rw [interpret_not hwI]
+  · rw [hiφ t₁ t₂ εs I hwt hwI]
+  · exact (hwφ t₁ t₂ εs hwt).left
+
+private theorem verifyEvaluatePair_ok_implies {φ : Term → Term → Term} {p₁ p₂ : Policy} {εnv : SymEnv} {asserts : Asserts} :
+  verifyEvaluatePair φ p₁ p₂ εnv = .ok asserts →
+  ∃ t₁ t₂ ts,
+    compile p₁.toExpr εnv = .ok t₁ ∧
+    compile p₂.toExpr εnv = .ok t₂ ∧
+    enforce [p₁.toExpr, p₂.toExpr] εnv = Set.mk ts ∧
+    asserts = ts ++ [not (φ t₁ t₂)]
+:= by
+  intro hok
+  simp only [verifyEvaluatePair] at hok
+  simp_do_let (compile p₁.toExpr εnv) at hok
+  simp_do_let (compile p₂.toExpr εnv) at hok
+  simp only [Except.ok.injEq] at hok
+  subst hok
+  rename_i t₁ hr₁ t₂ hr₂
+  exists t₁, t₂, (enforce [p₁.toExpr, p₂.toExpr] εnv).elts
+
+theorem verifyEvaluatePair_is_sound {φ : Term → Term → Term} {f : Spec.Result Value → Spec.Result Value → Bool} {p₁ p₂ : Policy} {εnv : SymEnv} {asserts : Asserts} :
+  WellBehavedEvaluatePairQuery φ f →
+  εnv.StronglyWellFormedForPolicy p₁ →
+  εnv.StronglyWellFormedForPolicy p₂ →
+  verifyEvaluatePair φ p₁ p₂ εnv = .ok asserts →
+  εnv ⊭ asserts →
+  ∀ env,
+    env ∈ᵢ εnv →
+    env.StronglyWellFormedForPolicy p₁ →
+    env.StronglyWellFormedForPolicy p₂ →
+    f (evaluate p₁.toExpr env.request env.entities) (evaluate p₂.toExpr env.request env.entities) = true
+:= by
+  intro ⟨hwφ, hiφ, hφf⟩ hwε₁ hwε₂ hok hsat env ⟨I, hwI, heq⟩ hwe₁ hwe₂
+  rw [asserts_unsatisfiable_def] at hsat
+  replace ⟨t, hsat⟩ := hsat I hwI
+  replace ⟨t₁, t₂, ts, hok₁, hok₂, ha, hvc⟩ := verifyEvaluatePair_ok_implies hok
+  subst hvc
+  replace ha := swf_implies_enforce_satisfiedBy heq hwI
+    (swf_εnv_for_policies_iff_swf_for_append.mp (And.intro
+      (swf_εnv_for_policy_iff_swf_for_polices.mp hwε₁)
+      (swf_εnv_for_policy_iff_swf_for_polices.mp hwε₂)))
+    (swf_env_for_policies_iff_swf_for_append.mp (And.intro
+      (swf_env_for_policy_iff_swf_for_polices.mp hwe₁)
+      (swf_env_for_policy_iff_swf_for_polices.mp hwe₂))) ha
+  replace ha := asserts_last_not_true ha hsat.left hsat.right
+  subst ha
+  simp only [List.mem_append, List.mem_cons, List.not_mem_nil, or_false, or_true, ne_eq, true_and] at hsat
+  replace hwε₁ := swf_εnv_for_implies_wf_for hwε₁
+  replace hwε₂ := swf_εnv_for_implies_wf_for hwε₂
+  replace hwe₁ := swf_env_for_implies_wf_for hwe₁
+  replace hwe₂ := swf_env_for_implies_wf_for hwe₂
+  have hrb₁ := compile_bisimulation hwε₁ hwe₁ hwI heq hok₁
+  have hrb₂ := compile_bisimulation hwε₂ hwe₂ hwI heq hok₂
+  have hwt₁ := compile_policy_wf hwε₁ hok₁
+  have hwt₂ := compile_policy_wf hwε₂ hok₂
+  rw [interpret_not_wbepq hwI ⟨hwt₁.left, hwt₁.right, hwt₂.left, hwt₂.right⟩ hwφ hiφ] at hsat
+  replace hrb := wbepq_bisimulation ⟨hwt₁.left, hwt₁.right, hwt₂.left, hwt₂.right⟩ hφf hwI hrb₁ hrb₂
+  exact same_bool_not_not_true_implies_true hrb hsat
+
+theorem verifyEvaluatePair_is_complete {φ : Term → Term → Term} {f : Spec.Result Value → Spec.Result Value → Bool} {p₁ p₂ : Policy} {εnv : SymEnv} {asserts : Asserts} :
+  WellBehavedEvaluatePairQuery φ f →
+  εnv.StronglyWellFormedForPolicy p₁ →
+  εnv.StronglyWellFormedForPolicy p₂ →
+  verifyEvaluatePair φ p₁ p₂ εnv = .ok asserts →
+  εnv ⊧ asserts →
+  ∃ env,
+    env ∈ᵢ εnv ∧
+    env.StronglyWellFormedForPolicy p₁ ∧
+    env.StronglyWellFormedForPolicy p₂ ∧
+    Env.EnumCompleteFor env εnv ∧
+    f (evaluate p₁.toExpr env.request env.entities) (evaluate p₂.toExpr env.request env.entities) = false
+:= by
+  intro ⟨hwφ, hiφ, hφf⟩ hwε₁ hwε₂ hok hsat
+  rw [asserts_satisfiable_def] at hsat
+  replace ⟨I, hwI, hsat⟩ := hsat
+  replace ⟨t₁, t₂, ts, hok₁, hok₂, ha, hvc⟩ := verifyEvaluatePair_ok_implies hok
+  subst hvc
+  replace ⟨hsat, hvc⟩ := asserts_all_true hsat
+  replace ⟨I', env, hwI', heq, hwe, henum_comp, hsat⟩ := enforce_satisfiedBy_implies_exists_swf
+    (swf_εnv_for_policies_iff_swf_for_append.mp (And.intro
+      (swf_εnv_for_policy_iff_swf_for_polices.mp hwε₁)
+      (swf_εnv_for_policy_iff_swf_for_polices.mp hwε₂))) hwI ha hsat
+  exists env
+  rw [← swf_env_for_policies_iff_swf_for_append] at hwe
+  have hwe₁ : env.StronglyWellFormedForPolicy p₁ := by
+    have := hwe.left
+    rwa [← swf_env_for_policy_iff_swf_for_polices] at this
+  have hwe₂ : env.StronglyWellFormedForPolicy p₂ := by
+    have := hwe.right
+    rwa [← swf_env_for_policy_iff_swf_for_polices] at this
+  simp only [memOfSymEnv, hwe₁, hwe₂, true_and]
+  constructor
+  · exists I'
+  · replace hwε₁ := swf_εnv_for_implies_wf_for hwε₁
+    replace hwε₂ := swf_εnv_for_implies_wf_for hwε₂
+    replace hwe₁ := swf_env_for_implies_wf_for hwe₁
+    replace hwe₂ := swf_env_for_implies_wf_for hwe₂
+    have hrb₁ := compile_bisimulation hwε₁ hwe₁ hwI' heq hok₁
+    have hrb₂ := compile_bisimulation hwε₂ hwe₂ hwI' heq hok₂
+    have hwt₁ := compile_policy_wf hwε₁ hok₁
+    have hwt₂ := compile_policy_wf hwε₂ hok₂
+    have hsat₁ := hsat p₁ t₁ (by simp) hok₁
+    have hsat₂ := hsat p₂ t₂ (by simp) hok₂
+    rw [interpret_not_wbepq hwI ⟨hwt₁.left, hwt₁.right, hwt₂.left, hwt₂.right⟩ hwφ hiφ] at hvc
+    rw [hsat₁, hsat₂] at hvc
+    replace hrb := wbepq_bisimulation ⟨hwt₁.left, hwt₁.right, hwt₂.left, hwt₂.right⟩ hφf hwI' hrb₁ hrb₂
+    simp only [henum_comp, true_and]
+    exact same_bool_not_true_implies_false hrb hvc
+
+end Cedar.Thm
