cedar-lean/Cedar/Thm/SymCC/Verifier/VerifyEvaluatePairQueries.lean
@@ -1,0 +1,345 @@
+/-
+ Copyright Cedar Contributors
+
+ Licensed under the Apache License, Version 2.0 (the "License");
+ you may not use this file except in compliance with the License.
+ You may obtain a copy of the License at
+
+      https://www.apache.org/licenses/LICENSE-2.0
+
+ Unless required by applicable law or agreed to in writing, software
+ distributed under the License is distributed on an "AS IS" BASIS,
+ WITHOUT WARRANTIES OR CONDITIONS OF ANY KIND, either express or implied.
+ See the License for the specific language governing permissions and
+ limitations under the License.
+-/
+
+import Cedar.Thm.SymCC.Verifier.VerifyEvaluatePair
+import Cedar.Thm.SymCC.Verifier.VerifyEvaluateQueries
+
+/-!
+This file proves that `verifyEvaluatePair` queries are well-behaved.
+--/
+
+namespace Cedar.Thm
+
+open Data Spec SymCC Factory
+
+@[simp]
+private theorem error_beq_ok [BEq ε] [LawfulBEq ε] [BEq α] [LawfulBEq α] (e : ε) (v : α) :
+  (Except.error e == Except.ok v) = false
+:= by simp
+
+@[simp]
+private theorem ok_beq_ok [BEq ε] [LawfulBEq ε] [BEq α] [LawfulBEq α] (v₁ v₂ : α) :
+  (Except.ok v₁ == Except.ok v₂ (ε := ε)) = (v₁ == v₂)
+:= by
+  by_cases v₁ = v₂
+  · subst v₂ ; simp
+  · simp [*, BEq.beq, instBEqExcept_cedar.beq]
+
+@[simp]
+private theorem ok_ne_ok [BEq ε] [LawfulBEq ε] [BEq α] [LawfulBEq α] (v₁ v₂ : α) :
+  Except.ok v₁ ≠ Except.ok v₂ (ε := ε) ↔ v₁ ≠ v₂
+:= by simp
+
+theorem verifyMatchesEquivalent_wbepq :
+  WellBehavedEvaluatePairQuery
+    (λ t₁ t₂ =>
+      let t₁matches := eq t₁ (⊙true)
+      let t₂matches := eq t₂ (⊙true)
+      eq t₁matches t₂matches)
+    (λ r₁ r₂ => (r₁ == .ok true) == (r₂ == .ok true))
+:= by
+  constructor
+  · -- WellFormedOutput
+    simp only [WellBehavedEvaluatePairQuery.WellFormedOutput]
+    intro t₁ t₂ εs ⟨hwt₁, hty₁, hwt₂, hty₂⟩
+    have hwf₁ := wf_eq hwt₁ (Term.WellFormed.some_wf (wf_bool (b := true)))
+      (by rw [hty₁]; simp only [typeOf_term_some, Term.typeOf, TermPrim.typeOf])
+    have hwf₂ := wf_eq hwt₂ (Term.WellFormed.some_wf (wf_bool (b := true)))
+      (by rw [hty₂]; simp only [typeOf_term_some, Term.typeOf, TermPrim.typeOf])
+    exact wf_eq hwf₁.left hwf₂.left (by simp only [someOf]; rw [hwf₁.right, hwf₂.right])
+  constructor
+  · -- Interpretable
+    simp only [WellBehavedEvaluatePairQuery.Interpretable]
+    intro t₁ t₂ εs I ⟨hwt₁, hty₁, hwt₂, hty₂⟩ hwI
+    have hwf₁ := wf_eq hwt₁ (Term.WellFormed.some_wf (wf_bool (b := true)))
+      (by rw [hty₁]; simp only [typeOf_term_some, Term.typeOf, TermPrim.typeOf])
+    have hwf₂ := wf_eq hwt₂ (Term.WellFormed.some_wf (wf_bool (b := true)))
+      (by rw [hty₂]; simp only [typeOf_term_some, Term.typeOf, TermPrim.typeOf])
+    simp only [someOf]
+    rw [interpret_eq hwI hwf₁.left hwf₂.left,
+        interpret_eq hwI hwt₁ (Term.WellFormed.some_wf (wf_bool (b := true))),
+        interpret_eq hwI hwt₂ (Term.WellFormed.some_wf (wf_bool (b := true)))]
+    simp only [interpret_term_some, interpret_term_prim]
+  · -- Same
+    intro t₁ t₂ εs r₁ r₂ ⟨hwt₁, hty₁, hwt₂, hty₂⟩ hs₁ hs₂
+    cases r₁ <;> cases r₂
+    case error.error =>
+      replace ⟨_, hs₁⟩ := (same_error_implies hs₁).right
+      replace ⟨_, hs₂⟩ := (same_error_implies hs₂).right
+      subst hs₁ hs₂
+      simp only [same_bool_def, someOf, pe_eq_none_some]
+      rfl
+    case error.ok =>
+      replace ⟨_, hs₁⟩ := (same_error_implies hs₁).right
+      replace ⟨t₂', heq₂, hs₂⟩ := same_ok_implies hs₂
+      subst hs₁ heq₂
+      have hwt₂' : t₂'.WellFormed εs ∧ t₂'.typeOf = .bool := by
+        constructor
+        · exact wf_term_some_implies hwt₂
+        · rw [typeOf_term_some, TermType.option.injEq] at hty₂
+          exact hty₂
+      replace ⟨b₂, hv₂⟩ := value_type_bool_implies_bool hs₂ hwt₂'.right
+      subst hv₂
+      replace hs₂ := same_bool_implies hs₂
+      subst hs₂
+      simp only [same_bool_def, someOf, pe_eq_none_some, pe_eq_some_some]
+      cases b₂ <;> simp only [pe_eq_simplify_same, pe_eq_simplify_lit, term_prim_is_lit, pe_eq_prim, error_beq_ok]
+      · have : (Term.prim (.bool false) == Term.prim (.bool true)) = false := by simp
+        simp [this]
+      · simp
+    case ok.error =>
+      replace ⟨t₁', heq₁, hs₁⟩ := same_ok_implies hs₁
+      replace ⟨_, hs₂⟩ := (same_error_implies hs₂).right
+      subst heq₁ hs₂
+      have hwt₁' : t₁'.WellFormed εs ∧ t₁'.typeOf = .bool := by
+        constructor
+        · exact wf_term_some_implies hwt₁
+        · rw [typeOf_term_some, TermType.option.injEq] at hty₁
+          exact hty₁
+      replace ⟨b₁, hv₁⟩ := value_type_bool_implies_bool hs₁ hwt₁'.right
+      subst hv₁
+      replace hs₁ := same_bool_implies hs₁
+      rw [hs₁]
+      simp only [same_bool_def, someOf, pe_eq_some_some, pe_eq_none_some]
+      cases b₁ <;> simp only [pe_eq_simplify_same, pe_eq_simplify_lit, term_prim_is_lit, pe_eq_prim, error_beq_ok]
+      · have : (Term.prim (.bool false) == Term.prim (.bool true)) = false := by simp
+        simp [this]
+      · simp
+    case ok.ok =>
+      replace ⟨t₁', heq₁, hs₁⟩ := same_ok_implies hs₁
+      replace ⟨t₂', heq₂, hs₂⟩ := same_ok_implies hs₂
+      subst heq₁ heq₂
+      have hwt₁' : t₁'.WellFormed εs ∧ t₁'.typeOf = .bool := by
+        constructor
+        · exact wf_term_some_implies hwt₁
+        · rw [typeOf_term_some, TermType.option.injEq] at hty₁
+          exact hty₁
+      have hwt₂' : t₂'.WellFormed εs ∧ t₂'.typeOf = .bool := by
+        constructor
+        · exact wf_term_some_implies hwt₂
+        · rw [typeOf_term_some, TermType.option.injEq] at hty₂
+          exact hty₂
+      replace ⟨b₁, hv₁⟩ := value_type_bool_implies_bool hs₁ hwt₁'.right
+      replace ⟨b₂, hv₂⟩ := value_type_bool_implies_bool hs₂ hwt₂'.right
+      subst hv₁ hv₂
+      replace hs₁ := same_bool_implies hs₁
+      replace hs₂ := same_bool_implies hs₂
+      rw [hs₁, hs₂]
+      simp only [same_bool_def, someOf, pe_eq_some_some]
+      cases b₁ <;> cases b₂ <;> simp only [pe_eq_simplify_same, pe_eq_simplify_lit, term_prim_is_lit, pe_eq_prim]
+      · have : (Term.prim (.bool false) == Term.prim (.bool true)) = false := by simp
+        simp [this]
+      · simp [BEq.beq, instBEqExcept_cedar.beq]
+      · simp [BEq.beq, instBEqExcept_cedar.beq]
+      · simp [BEq.beq, instBEqExcept_cedar.beq]
+
+theorem verifyMatchesImplies_wbepq :
+  WellBehavedEvaluatePairQuery
+    (λ t₁ t₂ =>
+      let t₁matches := eq t₁ (⊙true)
+      let t₂matches := eq t₂ (⊙true)
+      implies t₁matches t₂matches)
+    (λ r₁ r₂ => (r₁ != .ok true) || (r₂ == .ok true))
+:= by
+  constructor
+  · -- WellFormedOutput
+    simp only [WellBehavedEvaluatePairQuery.WellFormedOutput]
+    intro t₁ t₂ εs ⟨hwt₁, hty₁, hwt₂, hty₂⟩
+    have hwf₁ := wf_eq hwt₁ (Term.WellFormed.some_wf (wf_bool (b := true)))
+      (by rw [hty₁]; simp only [typeOf_term_some, Term.typeOf, TermPrim.typeOf])
+    have hwf₂ := wf_eq hwt₂ (Term.WellFormed.some_wf (wf_bool (b := true)))
+      (by rw [hty₂]; simp only [typeOf_term_some, Term.typeOf, TermPrim.typeOf])
+    simp only [implies]
+    have hwf_not := wf_not hwf₁.left hwf₁.right
+    exact wf_or hwf_not.left hwf₂.left hwf_not.right hwf₂.right
+  constructor
+  · -- Interpretable
+    simp only [WellBehavedEvaluatePairQuery.Interpretable]
+    intro t₁ t₂ εs I ⟨hwt₁, hty₁, hwt₂, hty₂⟩ hwI
+    have hwf₁ := wf_eq hwt₁ (Term.WellFormed.some_wf (wf_bool (b := true)))
+      (by rw [hty₁]; simp only [typeOf_term_some, Term.typeOf, TermPrim.typeOf])
+    have hwf₂ := wf_eq hwt₂ (Term.WellFormed.some_wf (wf_bool (b := true)))
+      (by rw [hty₂]; simp only [typeOf_term_some, Term.typeOf, TermPrim.typeOf])
+    have hwf_not := wf_not hwf₁.left hwf₁.right
+    simp only [implies, someOf]
+    rw [interpret_or hwI hwf_not.left hwf₂.left hwf_not.right hwf₂.right,
+        interpret_not hwI hwf₁.left,
+        interpret_eq hwI hwt₁ (Term.WellFormed.some_wf (wf_bool (b := true))),
+        interpret_eq hwI hwt₂ (Term.WellFormed.some_wf (wf_bool (b := true)))]
+    simp only [interpret_term_some, interpret_term_prim]
+  · -- Same
+    intro t₁ t₂ εs r₁ r₂ ⟨hwt₁, hty₁, hwt₂, hty₂⟩ hs₁ hs₂
+    cases r₁ <;> cases r₂
+    case error.error =>
+      replace ⟨_, hs₁⟩ := (same_error_implies hs₁).right
+      replace ⟨_, hs₂⟩ := (same_error_implies hs₂).right
+      subst hs₁ hs₂
+      simp only [same_bool_def, someOf, implies, pe_eq_none_some, pe_not_lit]
+      rfl
+    case error.ok =>
+      replace ⟨_, hs₁⟩ := (same_error_implies hs₁).right
+      replace ⟨t₂', heq₂, hs₂⟩ := same_ok_implies hs₂
+      subst hs₁ heq₂
+      have hwt₂' : t₂'.WellFormed εs ∧ t₂'.typeOf = .bool := by
+        constructor
+        · exact wf_term_some_implies hwt₂
+        · rw [typeOf_term_some, TermType.option.injEq] at hty₂
+          exact hty₂
+      replace ⟨b₂, hv₂⟩ := value_type_bool_implies_bool hs₂ hwt₂'.right
+      subst hv₂
+      replace hs₂ := same_bool_implies hs₂
+      subst hs₂
+      simp only [same_bool_def, someOf, implies, pe_eq_none_some, pe_eq_some_some]
+      cases b₂ <;> simp [pe_eq_simplify_same, pe_eq_simplify_lit, term_prim_is_lit, pe_not_lit, pe_or_true_left]
+    case ok.error =>
+      replace ⟨t₁', heq₁, hs₁⟩ := same_ok_implies hs₁
+      replace ⟨_, hs₂⟩ := (same_error_implies hs₂).right
+      subst heq₁ hs₂
+      have hwt₁' : t₁'.WellFormed εs ∧ t₁'.typeOf = .bool := by
+        constructor
+        · exact wf_term_some_implies hwt₁
+        · rw [typeOf_term_some, TermType.option.injEq] at hty₁
+          exact hty₁
+      replace ⟨b₁, hv₁⟩ := value_type_bool_implies_bool hs₁ hwt₁'.right
+      subst hv₁
+      replace hs₁ := same_bool_implies hs₁
+      rw [hs₁]
+      simp only [same_bool_def, someOf, implies, pe_eq_some_some, pe_eq_none_some]
+      cases b₁ <;> simp [pe_eq_simplify_same, pe_eq_simplify_lit, term_prim_is_lit, pe_not_lit, pe_or_false_right]
+      · simp [BEq.beq]
+    case ok.ok =>
+      replace ⟨t₁', heq₁, hs₁⟩ := same_ok_implies hs₁
+      replace ⟨t₂', heq₂, hs₂⟩ := same_ok_implies hs₂
+      subst heq₁ heq₂
+      have hwt₁' : t₁'.WellFormed εs ∧ t₁'.typeOf = .bool := by
+        constructor
+        · exact wf_term_some_implies hwt₁
+        · rw [typeOf_term_some, TermType.option.injEq] at hty₁
+          exact hty₁
+      have hwt₂' : t₂'.WellFormed εs ∧ t₂'.typeOf = .bool := by
+        constructor
+        · exact wf_term_some_implies hwt₂
+        · rw [typeOf_term_some, TermType.option.injEq] at hty₂
+          exact hty₂
+      replace ⟨b₁, hv₁⟩ := value_type_bool_implies_bool hs₁ hwt₁'.right
+      replace ⟨b₂, hv₂⟩ := value_type_bool_implies_bool hs₂ hwt₂'.right
+      subst hv₁ hv₂
+      replace hs₁ := same_bool_implies hs₁
+      replace hs₂ := same_bool_implies hs₂
+      rw [hs₁, hs₂]
+      simp only [same_bool_def, someOf, implies, pe_eq_some_some]
+      have : (Term.prim (.bool false) == Term.prim (.bool true)) = false := by simp
+      cases b₁ <;> cases b₂ <;> simp [pe_eq_simplify_same, pe_eq_simplify_lit, term_prim_is_lit, pe_not_lit, pe_or_true_right, pe_or_false_right, this]
+
+theorem verifyMatchesDisjoint_wbepq :
+  WellBehavedEvaluatePairQuery
+    (λ t₁ t₂ =>
+      let t₁matches := eq t₁ (⊙true)
+      let t₂matches := eq t₂ (⊙true)
+      not (and t₁matches t₂matches))
+    (λ r₁ r₂ => !((r₁ == .ok true) && (r₂ == .ok true)))
+:= by
+  constructor
+  · -- WellFormedOutput
+    simp only [WellBehavedEvaluatePairQuery.WellFormedOutput]
+    intro t₁ t₂ εs ⟨hwt₁, hty₁, hwt₂, hty₂⟩
+    have hwf₁ := wf_eq hwt₁ (Term.WellFormed.some_wf (wf_bool (b := true)))
+      (by rw [hty₁]; simp only [typeOf_term_some, Term.typeOf, TermPrim.typeOf])
+    have hwf₂ := wf_eq hwt₂ (Term.WellFormed.some_wf (wf_bool (b := true)))
+      (by rw [hty₂]; simp only [typeOf_term_some, Term.typeOf, TermPrim.typeOf])
+    have hwf_and := wf_and hwf₁.left hwf₂.left hwf₁.right hwf₂.right
+    exact wf_not hwf_and.left hwf_and.right
+  constructor
+  · -- Interpretable
+    simp only [WellBehavedEvaluatePairQuery.Interpretable]
+    intro t₁ t₂ εs I ⟨hwt₁, hty₁, hwt₂, hty₂⟩ hwI
+    have hwf₁ := wf_eq hwt₁ (Term.WellFormed.some_wf (wf_bool (b := true)))
+      (by rw [hty₁]; simp only [typeOf_term_some, Term.typeOf, TermPrim.typeOf])
+    have hwf₂ := wf_eq hwt₂ (Term.WellFormed.some_wf (wf_bool (b := true)))
+      (by rw [hty₂]; simp only [typeOf_term_some, Term.typeOf, TermPrim.typeOf])
+    have hwf_and := wf_and hwf₁.left hwf₂.left hwf₁.right hwf₂.right
+    simp only [someOf]
+    rw [interpret_not hwI hwf_and.left,
+        interpret_and hwI hwf₁.left hwf₂.left hwf₁.right hwf₂.right,
+        interpret_eq hwI hwt₁ (Term.WellFormed.some_wf (wf_bool (b := true))),
+        interpret_eq hwI hwt₂ (Term.WellFormed.some_wf (wf_bool (b := true)))]
+    simp only [interpret_term_some, interpret_term_prim]
+  · -- Same
+    intro t₁ t₂ εs r₁ r₂ ⟨hwt₁, hty₁, hwt₂, hty₂⟩ hs₁ hs₂
+    cases r₁ <;> cases r₂
+    case error.error =>
+      replace ⟨_, hs₁⟩ := (same_error_implies hs₁).right
+      replace ⟨_, hs₂⟩ := (same_error_implies hs₂).right
+      subst hs₁ hs₂
+      simp only [same_bool_def, someOf, pe_eq_none_some, pe_and_false_left, pe_not_false]
+      rfl
+    case error.ok =>
+      replace ⟨_, hs₁⟩ := (same_error_implies hs₁).right
+      replace ⟨t₂', heq₂, hs₂⟩ := same_ok_implies hs₂
+      subst hs₁ heq₂
+      have hwt₂' : t₂'.WellFormed εs ∧ t₂'.typeOf = .bool := by
+        constructor
+        · exact wf_term_some_implies hwt₂
+        · rw [typeOf_term_some, TermType.option.injEq] at hty₂
+          exact hty₂
+      replace ⟨b₂, hv₂⟩ := value_type_bool_implies_bool hs₂ hwt₂'.right
+      subst hv₂
+      replace hs₂ := same_bool_implies hs₂
+      subst hs₂
+      simp only [same_bool_def, someOf, pe_eq_none_some, pe_eq_some_some]
+      cases b₂ <;> simp [pe_eq_simplify_same, pe_eq_simplify_lit, term_prim_is_lit, pe_and_false_left, pe_not_false]
+    case ok.error =>
+      replace ⟨t₁', heq₁, hs₁⟩ := same_ok_implies hs₁
+      replace ⟨_, hs₂⟩ := (same_error_implies hs₂).right
+      subst heq₁ hs₂
+      have hwt₁' : t₁'.WellFormed εs ∧ t₁'.typeOf = .bool := by
+        constructor
+        · exact wf_term_some_implies hwt₁
+        · rw [typeOf_term_some, TermType.option.injEq] at hty₁
+          exact hty₁
+      replace ⟨b₁, hv₁⟩ := value_type_bool_implies_bool hs₁ hwt₁'.right
+      subst hv₁
+      replace hs₁ := same_bool_implies hs₁
+      rw [hs₁]
+      simp only [same_bool_def, someOf, pe_eq_some_some, pe_eq_none_some]
+      cases b₁ <;> simp only [pe_eq_simplify_same, pe_eq_simplify_lit, term_prim_is_lit, pe_and_false_right, pe_not_false]
+      · simp [Bool.and_false, Bool.not_false]
+      · simp [Bool.and_false, Bool.not_false]
+    case ok.ok =>
+      replace ⟨t₁', heq₁, hs₁⟩ := same_ok_implies hs₁
+      replace ⟨t₂', heq₂, hs₂⟩ := same_ok_implies hs₂
+      subst heq₁ heq₂
+      have hwt₁' : t₁'.WellFormed εs ∧ t₁'.typeOf = .bool := by
+        constructor
+        · exact wf_term_some_implies hwt₁
+        · rw [typeOf_term_some, TermType.option.injEq] at hty₁
+          exact hty₁
+      have hwt₂' : t₂'.WellFormed εs ∧ t₂'.typeOf = .bool := by
+        constructor
+        · exact wf_term_some_implies hwt₂
+        · rw [typeOf_term_some, TermType.option.injEq] at hty₂
+          exact hty₂
+      replace ⟨b₁, hv₁⟩ := value_type_bool_implies_bool hs₁ hwt₁'.right
+      replace ⟨b₂, hv₂⟩ := value_type_bool_implies_bool hs₂ hwt₂'.right
+      subst hv₁ hv₂
+      replace hs₁ := same_bool_implies hs₁
+      replace hs₂ := same_bool_implies hs₂
+      rw [hs₁, hs₂]
+      simp only [same_bool_def, someOf, pe_eq_some_some]
+      have : (Term.prim (.bool false) == Term.prim (.bool true)) = false := by simp
+      cases b₁ <;> cases b₂ <;> simp [pe_eq_simplify_same, pe_eq_simplify_lit, term_prim_is_lit, pe_and_false_left, pe_and_false_right, pe_and_true_left, pe_not_false, pe_not_true, this]
+
+end Cedar.Thm
